A little more work on stack correctness

02Stack/Stack.thy
@@ -23,13 +23,6 @@ datatype focus =
 
 datatype stack_state = StackState focus "frame list" "expr heap"
 
-primrec devalue :: "val \<Rightarrow> expr" where
-  "devalue (VAbs t e) = Abs t e"
-| "devalue (VRec xs) = Rec xs"
-| "devalue (VInj l ts x) = Inj l ts x"
-| "devalue (VFold t x) = Fold t x"
-| "devalue (VTyAbs k e) = TyAbs k e"
-
 primrec free_vars\<^sub>s :: "frame \<Rightarrow> nat set" where
   "free_vars\<^sub>s (SRef x) = {x}"
 | "free_vars\<^sub>s (SApp e) = free_vars e"
@@ -41,5 +34,33 @@ primrec free_vars\<^sub>s :: "frame \<Rightarrow> nat set" where
 primrec free_vars\<^sub>s\<^sub>s :: "frame list \<Rightarrow> nat set" where
   "free_vars\<^sub>s\<^sub>s [] = {}"
 | "free_vars\<^sub>s\<^sub>s (f # s) = free_vars\<^sub>s f \<union> free_vars\<^sub>s\<^sub>s s"
+
+primrec devalue :: "val \<Rightarrow> expr" where
+  "devalue (VAbs t e) = Abs t e"
+| "devalue (VRec xs) = Rec xs"
+| "devalue (VInj l ts x) = Inj l ts x"
+| "devalue (VFold t x) = Fold t x"
+| "devalue (VTyAbs k e) = TyAbs k e"
+
+primrec revalue :: "expr \<Rightarrow> val \<times> expr list" where
+  "revalue (Var x) = undefined "
+| "revalue (Abs t e) = (VAbs t e, [])"
+| "revalue (App e\<^sub>1 e\<^sub>2) = undefined"
+| "revalue (Let e\<^sub>1 e\<^sub>2) = (case revalue e\<^sub>2 of (v, bs) \<Rightarrow> (v, e\<^sub>1 # bs))"
+| "revalue (Rec xs) = (VRec xs, [])"
+| "revalue (Proj e l) = undefined"
+| "revalue (Inj l ts x) = (VInj l ts x, [])"
+| "revalue (Case e t cs) = undefined"
+| "revalue (Fold t x) = (VFold t x, [])"
+| "revalue (Unfold t e) = undefined"
+| "revalue (TyAbs k e) = (VTyAbs k e, [])"
+| "revalue (TyApp e t) = undefined"
+| "revalue (TyLet t e) = undefined"
+
+lemma [simp]: "revalue (devalue v) = (v, [])"
+  by (induction v) simp_all
+
+lemma [simp]: "is_value e \<Longrightarrow> revalue e = (v, bs) \<Longrightarrow> foldr Let bs (devalue v) = e"
+  by (induction e arbitrary: bs) (auto split: prod.splits)
 
 end
