Utilities/Iterate.thy
@@ -2,8 +2,11 @@ theory Iterate
 imports Main
 begin
 
-inductive iter :: "('a \<Rightarrow> 'a \<Rightarrow> bool) \<Rightarrow> ('a \<Rightarrow> 'a \<Rightarrow> bool)" where
+inductive iter :: "('a \<Rightarrow> 'a \<Rightarrow> bool) \<Rightarrow> ('a \<Rightarrow> 'a \<Rightarrow> bool)" for f where
   iter_refl [simp]: "iter f a a"
 | iter_step [simp]: "f a b \<Longrightarrow> iter f b c \<Longrightarrow> iter f a c"
+
+lemma [elim]: "iter f a b \<Longrightarrow> iter f b c \<Longrightarrow> iter f a c"
+  by (induction a b rule: iter.induct) simp_all
 
 end
