02Stack/StackCorrectness.thy
@@ -2,16 +2,121 @@ theory StackCorrectness
 imports StackConversion "../01Expression/Evaluate" "../Utilities/Iterate"
 begin
 
-lemma complete: "iter (op \<leadsto>) e e' \<Longrightarrow> 
-    \<exists>\<Sigma> \<Sigma>'. iter (op \<leadsto>\<^sub>s) \<Sigma> \<Sigma>' \<and> unstack_state \<Sigma> e \<and> unstack_state \<Sigma>' e'"
-  by simp
+lemma complete': "e \<leadsto> e' \<Longrightarrow> unstack_state \<Sigma> e \<Longrightarrow> \<exists>\<Sigma>'. \<Sigma> \<leadsto>\<^sub>s \<Sigma>' \<and> unstack_state \<Sigma>' e'"
+  proof (induction e e' rule: evaluate.induct) 
+  case ev_app1
+    thus ?case by simp 
+  next case ev_app2 
+    thus ?case by simp 
+  next case ev_app_let
+    thus ?case by simp 
+  next case ev_let1
+    thus ?case by simp 
+  next case ev_let2
+    thus ?case by simp 
+  next case ev_let3
+    thus ?case by simp 
+  next case ev_proj1
+    thus ?case by simp 
+  next case ev_proj2 
+    thus ?case by simp 
+  next case ev_proj_let
+    thus ?case by simp 
+  next case ev_case1 
+    thus ?case by simp 
+  next case ev_case2
+    thus ?case by simp 
+  next case ev_case_let
+    thus ?case by simp 
+  next case ev_unfold1
+    thus ?case by simp 
+  next case ev_unfold2
+    thus ?case by simp 
+  next case ev_unfold_let
+    thus ?case by simp 
+  next case ev_tyapp1
+    thus ?case by simp 
+  next case ev_tyapp2
+    thus ?case by simp 
+  next case ev_tyapp_let
+    thus ?case by simp 
+  next case ev_tylet
+    thus ?case by simp 
+  qed 
 
-lemma sound: "iter (op \<leadsto>\<^sub>s) \<Sigma> \<Sigma>' \<Longrightarrow> 
-    \<exists>e e'. iter (op \<leadsto>) e e' \<and> unstack_state \<Sigma> e \<and> unstack_state \<Sigma>' e'"
-  by simp
+lemma complete: "iter (op \<leadsto>) e e' \<Longrightarrow> unstack_state \<Sigma> e \<Longrightarrow>
+    \<exists>\<Sigma>'. iter (op \<leadsto>\<^sub>s) \<Sigma> \<Sigma>' \<and> unstack_state \<Sigma>' e'"
+  proof (induction e e' arbitrary: \<Sigma> rule: iter.induct)
+  case iter_refl
+    thus ?case by (metis iter.iter_refl)
+  next case (iter_step e e' e'')
+    then obtain \<Sigma>' where "\<Sigma> \<leadsto>\<^sub>s \<Sigma>' \<and> unstack_state \<Sigma>' e'" by (metis complete')
+    moreover with iter_step obtain \<Sigma>'' where "iter (op \<leadsto>\<^sub>s) \<Sigma>' \<Sigma>'' \<and> unstack_state \<Sigma>'' e''" 
+      by fastforce
+    ultimately have "iter (op \<leadsto>\<^sub>s) \<Sigma> \<Sigma>'' \<and> unstack_state \<Sigma>'' e''" by fastforce
+    thus ?case by fastforce
+  qed
 
-theorem correct: "iter (op \<leadsto>) e e' \<Longrightarrow> is_value e' \<Longrightarrow> \<exists>v h. e' = devalue v \<and> 
-    iter (op \<leadsto>\<^sub>s) (StackState (Eval e) [] empty\<^sub>h) (StackState (Return v) [] h)"
-  by simp
+lemma sound': "\<Sigma> \<leadsto>\<^sub>s \<Sigma>' \<Longrightarrow> unstack_state \<Sigma> e \<Longrightarrow> \<exists>e'. iter (op \<leadsto>) e e' \<and> unstack_state \<Sigma>' e'"
+  proof (induction \<Sigma> \<Sigma>' arbitrary: e rule: EvaluateStack.evaluate.induct)
+  case (ev_var x s h)
+    hence "unstack_state (StackState (Eval (Var x)) s h) e" by simp
+
+
+have "unstack {} s (Var x) h {x. x < length\<^sub>h h} [] e \<Longrightarrow> 
+    unstack_state (StackState (Eval (Var x)) s h) e" by simp
+
+    have "\<exists>e'. iter op \<leadsto> e e' \<and> unstack_state (StackState (Eval (lookup\<^sub>h x h)) (SRef x # s) h) e'" by simp
+    thus ?case by simp
+  next case ev_abs 
+    thus ?case by simp
+  next case ev_app 
+    thus ?case by simp
+  next case ev_let 
+    thus ?case by simp
+  next case ev_rec 
+    thus ?case by simp
+  next case ev_proj 
+    thus ?case by simp
+  next case ev_inj 
+    thus ?case by simp
+  next case ev_case 
+    thus ?case by simp
+  next case ev_fold 
+    thus ?case by simp
+  next case ev_unfold 
+    thus ?case by simp
+  next case ev_tyabs 
+    thus ?case by simp
+  next case ev_tyapp 
+    thus ?case by simp
+  next case ev_tylet 
+    thus ?case by simp
+  next case ret_ref 
+    thus ?case by simp
+  next case ret_app 
+    thus ?case by simp
+  next case ret_proj 
+    thus ?case by simp
+  next case ret_case 
+    thus ?case by simp
+  next case ret_unfold 
+    thus ?case by simp
+  next case ret_tyapp 
+    thus ?case by simp
+  qed 
+
+lemma sound: "iter (op \<leadsto>\<^sub>s) \<Sigma> \<Sigma>' \<Longrightarrow> unstack_state \<Sigma> e \<Longrightarrow>
+    \<exists>e'. iter (op \<leadsto>) e e' \<and> unstack_state \<Sigma>' e'"
+  proof (induction \<Sigma> \<Sigma>' arbitrary: e rule: iter.induct)
+  case iter_refl
+    thus ?case by (metis iter.iter_refl)
+  next case (iter_step \<Sigma> \<Sigma>' \<Sigma>'')
+    then obtain e' where "iter (op \<leadsto>) e e' \<and> unstack_state \<Sigma>' e'" by (metis sound')
+    moreover with iter_step obtain e'' where "iter (op \<leadsto>) e' e'' \<and> unstack_state \<Sigma>'' e''" 
+      by fastforce
+    ultimately have "iter (op \<leadsto>) e e'' \<and> unstack_state \<Sigma>'' e''" by fastforce
+    thus ?case by fastforce
+  qed
 
 end
