Total.thy
@@ -2,7 +2,8 @@ theory Total
 imports "01Expression/Determinism" "02Stack/StackDeterminism" "02Stack/StackCorrectness"
 begin
 
-
-
+theorem correct: "is_value e' \<Longrightarrow> revalue e' = (v, h) \<Longrightarrow> 
+    iter (op \<leadsto>) e e' = iter (op \<leadsto>\<^sub>s) (StackState (Eval e) [] empty\<^sub>h) (StackState (Return v) [] h)"
+  by simp
 
 end
